theories/case_studies/macros/check_no_overlap_spec.v
@@ -1,0 +1,99 @@
+From iris.proofmode Require Import proofmode.
+From cap_machine Require Import rules proofmode.
+From cap_machine Require Export check_no_overlap.
+
+Section Check_No_Overlap_spec.
+  Context
+    {Σ : gFunctors}
+      {ceriseg: ceriseG Σ}
+      {MP: MachineParameters}
+  .
+
+  Lemma check_no_overlap_spec
+    (rsrc1 rsrc2 r1 r2 : RegName)
+    (pc_p : Perm) (pc_g : Locality) (pc_b pc_e pc_a : Addr)
+    (w1 w2 : Word)
+    (p1 : Perm) (g1 : Locality) (b1 e1 a1 : Addr)
+    (p2 : Perm) (g2 : Locality) (b2 e2 a2 : Addr)
+    (φ : language.val cap_lang → iPropI Σ) :
+
+    let check_no_overlap := (check_no_overlap_instrs rsrc1 rsrc2 r1 r2) in
+    let a_last := (pc_a ^+ length check_no_overlap)%a in
+    executeAllowed pc_p = true →
+    SubBounds pc_b pc_e pc_a a_last →
+    rsrc1 ≠ cnull ->
+    rsrc2 ≠ cnull ->
+    r1 ≠ cnull ->
+    r2 ≠ cnull ->
+
+    ▷ PC ↦ᵣ WCap pc_p pc_g pc_b pc_e pc_a
+    ∗ ▷ rsrc1 ↦ᵣ (WCap p1 g1 b1 e1 a1)
+    ∗ ▷ rsrc2 ↦ᵣ (WCap p2 g2 b2 e2 a2)
+    ∗ ▷ r1 ↦ᵣ w1
+    ∗ ▷ r2 ↦ᵣ w2
+    ∗ ▷ codefrag pc_a check_no_overlap
+    ∗ ▷ ( PC ↦ᵣ WCap pc_p pc_g pc_b pc_e a_last
+          ∗ rsrc1 ↦ᵣ (WCap p1 g1 b1 e1 a1)
+          ∗ rsrc2 ↦ᵣ (WCap p2 g2 b2 e2 a2)
+          ∗ r1 ↦ᵣ WInt 0%Z
+          ∗ r2 ↦ᵣ WInt 0%Z
+          ∗ ⌜ (finz.seq_between b1 e1) ## (finz.seq_between b2 e2) ⌝
+          ∗ codefrag pc_a check_no_overlap
+            -∗ WP Seq (Instr Executable) {{ φ }}
+        )
+    ∗ ▷ φ FailedV
+    ⊢ WP Seq (Instr Executable) {{ φ }}.
+  Proof.
+    intros check_no_overlap a_last ; subst check_no_overlap a_last.
+    iIntros (Hvpc Hcont Hrsrc1_cnull Hrsrc2_cnull Hr1_cnull Hr2_cnull)
+      "(>HPC & >Hrsrc1 & >Hrsrc2 & >Hr1 & >Hr2 & >Hprog & Hφ & Hfailed)".
+    iDestruct (big_sepL2_length with "Hprog") as %Hlength.
+    codefrag_facts "Hprog".
+    rename H into HcontRegion; clear H0.
+    cbn.
+
+    iInstr "Hprog".
+    iInstr "Hprog".
+    iInstr "Hprog".
+    destruct (b1 <? b2)%Z eqn:H_b1_b2; iEval (cbn) in "Hr1".
+    - (* b1 < b2 *)
+      iInstr "Hprog".
+      iInstr "Hprog".
+      iInstr "Hprog".
+      iInstr "Hprog".
+      iInstr "Hprog".
+      destruct ( (e1 - 1 <? b2)%Z ) eqn:H_e1_b2 ; iEval (cbn) in "Hr1".
+      + iInstr "Hprog".
+        iInstr "Hprog".
+        iInstr "Hprog".
+        iInstr "Hprog".
+        iApply "Hφ"; iFrame.
+        iPureIntro.
+        intros a Ha Ha'.
+        rewrite !elem_of_finz_seq_between in Ha, Ha'.
+        solve_addr.
+      + iInstr "Hprog".
+        iInstr "Hprog".
+        wp_end; iApply "Hfailed".
+    - (* b2 <= b1 *)
+      iInstr "Hprog".
+      iInstr "Hprog".
+      iInstr "Hprog".
+      iInstr "Hprog".
+      iInstr "Hprog".
+      destruct ( (e2 - 1 <? b1)%Z ) eqn:H_e2_b1 ; iEval (cbn) in "Hr1".
+      + iInstr "Hprog".
+        iInstr "Hprog".
+        iInstr "Hprog".
+        iInstr "Hprog".
+        iApply "Hφ"; iFrame.
+        iPureIntro.
+        intros a Ha Ha'.
+        rewrite !elem_of_finz_seq_between in Ha, Ha'.
+        solve_addr.
+      + iInstr "Hprog".
+        iInstr "Hprog".
+        wp_end; iApply "Hfailed".
+  Qed.
+
+End Check_No_Overlap_spec.
