theories/case_studies/macros/checkints.v
@@ -1,0 +1,338 @@
+From iris.proofmode Require Import proofmode.
+From cap_machine Require Import rules proofmode.
+From cap_machine Require Import is_word_type lea_to_base.
+
+Section Checkints.
+  Context
+      {MP: MachineParameters}
+  .
+
+
+  Definition checkints_loop_instrs (r r1 r2 : RegName) : list Word :=
+    encodeInstrsW [Load r1 r]
+      ++ is_int_instrs r1 r2
+      ++ encodeInstrsW
+      [ (* is an integer *)
+        Lea r 1;
+        GetA r1 r;
+        GetE r2 r;
+        Lt r1 r1 r2;
+        (* if r1 -> 0 then a + 1 >= e, and we continue,
+        otherwise we jump back to the beginning of the loop *)
+        Jnz (- ((length (is_int_instrs r1 r2))+5))%Z r1
+      ].
+
+  Definition checkints_instrs (r r1 r2 : RegName) : list Word :=
+      lea_to_base_instrs r r1 r2
+      ++ encodeInstrsW [
+        GetB r1 r;
+        GetE r2 r;
+        Lt r1 r1 r2;
+        Sub r1 r1 1; (* invert result for the jump *)
+        Jnz (length (checkints_loop_instrs r r1 r2) + 1) r1]
+      ++ checkints_loop_instrs r r1 r2
+      ++ encodeInstrsW [
+        Mov r1 0;
+        Mov r2 0].
+
+  Definition checkints_loop_offset : Z :=
+    Eval vm_compute in
+      length ( lea_to_base_instrs PC PC PC)
+      + length (
+            encodeInstrsW [
+                GetB PC PC;
+                GetE PC PC;
+                Lt PC PC PC;
+                Sub PC PC 1; (* invert result for the jump *)
+                Jnz (length (checkints_loop_instrs PC PC PC) + 1) PC])
+  .
+End Checkints.
+
+Section Checkints_spec.
+  Context
+    {Σ : gFunctors}
+      {ceriseg: ceriseG Σ}
+      {MP: MachineParameters}
+  .
+
+  Lemma checkints_loop_spec
+    (r r1 r2 : RegName)
+    (pc_p : Perm) (pc_g : Locality) (pc_b pc_e pc_a : Addr)
+    (w1 w2 : Word) (l : list Addr) (ws : list Word)
+    (p : Perm) (g : Locality) (b e a : Addr)
+    (φ : language.val cap_lang → iPropI Σ) :
+
+    let checkints_loop := (checkints_loop_instrs r r1 r2) in
+    let a_last := (pc_a ^+ length (checkints_loop_instrs r r1 r2))%a in
+    executeAllowed pc_p = true →
+    SubBounds pc_b pc_e pc_a a_last →
+    l ≡ₚ (finz.seq_between b e) ->
+    (b <= a < e)%a ->
+    readAllowed p = true ->
+    Forall (λ w,
+              (∃ k, ws !! k = Some w ∧ (∃ a', l !! k = Some a' ∧ (b <= a' < a)%a ))
+              ->
+              ∃ z, w = WInt z) ws ->
+    r ≠ cnull ->
+    r1 ≠ cnull ->
+    r2 ≠ cnull ->
+
+    ▷ PC ↦ᵣ WCap pc_p pc_g pc_b pc_e pc_a
+    ∗ ▷ r ↦ᵣ (WCap p g b e a)
+    ∗ ▷ r1 ↦ᵣ w1
+    ∗ ▷ r2 ↦ᵣ w2
+    ∗ ▷ codefrag pc_a checkints_loop
+    ∗ ▷ ( [∗ list] a;v ∈ l;ws, a ↦ₐ v )
+    ∗ ▷ ( PC ↦ᵣ WCap pc_p pc_g pc_b pc_e a_last
+         ∗ r ↦ᵣ WCap p g b e (finz.max b e)
+         ∗ r1 ↦ᵣ WInt 0%Z
+         ∗ r2 ↦ᵣ WInt e%Z
+         ∗ ( [∗ list] a;v ∈ l;ws, a ↦ₐ v )
+         ∗ ⌜ Forall (λ w, ∃ z, w = WInt z) ws ⌝
+         ∗ codefrag pc_a checkints_loop
+         -∗ WP Seq (Instr Executable) {{ φ }}
+        )
+    ∗ □ (▷ (φ FailedV))
+    ⊢ WP Seq (Instr Executable) {{ v, φ v }}.
+  Proof.
+    intros checkints a_last ; subst checkints a_last.
+    iIntros (Hvpc Hcont Hl Hae Hra Hall Hrcnull Hr1cnull Hr2cnull)
+      "(>HPC & >Hr & >Hr1 & >Hr2 & >Hcode & >Hmem & Hφ & #Hfailed)".
+    iLöb as "IH" forall ( a Hae Hall w1 w2).
+    iDestruct (big_sepL2_length with "Hcode") as %Hlength.
+    iDestruct (big_sepL2_length with "Hmem") as %Hlength_mem.
+    codefrag_facts "Hcode".
+    iEval (cbn) in "HPC".
+
+    focus_block_0 "Hcode" as "Hcode" "Hcont"; iHide "Hcont" as hcont.
+    assert (a ∈ l) as Ha.
+    { setoid_rewrite Hl; by rewrite elem_of_finz_seq_between. }
+    rewrite elem_of_list_lookup in Ha; destruct Ha as [ka Ha].
+    pose proof Ha as Ha'.
+    apply take_drop_middle in Ha'; symmetry in Ha'.
+    set (la1 := take ka l).
+    set (la2 := drop (S ka) l).
+    (* rewrite Hla in Hlength_mem. *)
+    assert (exists lw1 w lw2, ws = lw1 ++ w :: lw2
+                         ∧ length lw1 = length la1
+                         ∧ length lw2 = length la2
+           ) as (lw1 & w & lw2 & Hlw & Hlw1 & Hlw2).
+    {
+      (* rewrite elem_of_list_lookup in Ha'; destruct Ha' as [ka Ha]. *)
+      assert (is_Some (ws !! ka)) as [wa Hwa].
+      { exists (ws !!! ka).
+        apply list_lookup_lookup_total_lt.
+        rewrite -Hlength_mem.
+        eapply lookup_lt_Some; eauto.
+      }
+      pose proof Hwa as Hwa'.
+      apply take_drop_middle in Hwa'.
+      exists (take ka ws), wa, ((drop (S ka)) ws).
+      split; first done.
+      split.
+      + subst la1.
+        rewrite length_take_le; last (eapply Nat.lt_le_incl, lookup_lt_Some; eauto).
+        rewrite length_take_le; last (eapply Nat.lt_le_incl, lookup_lt_Some; eauto).
+        done.
+      + subst la2.
+        rewrite !length_drop.
+        rewrite Hlength_mem.
+        done.
+    }
+    rewrite Ha' Hlw.
+    iDestruct ( big_sepL2_app' with "Hmem") as "[Hmem1 Hmem]"; auto.
+    iDestruct ( big_sepL2_cons with "Hmem") as "[Ha Hmem2]"; auto.
+    iInstr "Hcode".
+    { split; auto; solve_addr. }
+    iDestruct ( big_sepL2_cons (λ _ a v, a ↦ₐ v)%I with "[$Ha $Hmem2]") as "Hmem"; auto.
+    iDestruct ( big_sepL2_app (λ _ a v, a ↦ₐ v)%I with "[$Hmem1] [$Hmem]") as "Hmem"; auto.
+    rewrite - Ha' - Hlw.
+    subst hcont; unfocus_block "Hcode" "Hcont" as "Hcode".
+
+    focus_block 1 "Hcode" as a_checkint Ha_checkint "Hcode" "Hcont"; iHide "Hcont" as hcont.
+    iApply (is_int_spec with "[- $HPC $Hr1 $Hr2 $Hcode]"); eauto.
+    iSplitR "Hfailed"; last (iNext; iApply "Hfailed").
+    iNext; iIntros "(HPC & Hr1 & %Hz & Hr2 & Hcode)".
+    subst hcont; unfocus_block "Hcode" "Hcont" as "Hcode".
+
+    focus_block 2 "Hcode" as a_cond Ha_cond "Hcode" "Hcont"; iHide "Hcont" as hcont ; clear Ha_checkint a_checkint.
+    iInstr "Hcode".
+    { transitivity (Some (a^+1)%a); auto; solve_addr. }
+    iInstr "Hcode".
+    iInstr "Hcode".
+    iInstr "Hcode".
+    destruct (decide ((a + 1%nat)%Z < e)%Z) as [Hae' | Hae']; cycle 1.
+    - replace (a ^+ 1)%a with e by solve_addr.
+      replace (e <? e)%Z with false by solve_addr.
+      iInstr "Hcode".
+      subst hcont; unfocus_block "Hcode" "Hcont" as "Hcode".
+      replace (finz.max b e) with e by solve_addr.
+      replace (a_cond ^+ 5)%a with (pc_a ^+ length (checkints_loop_instrs r r1 r2))%a by solve_addr.
+      iApply "Hφ"; iFrame; eauto.
+      iPureIntro.
+      apply Forall_forall.
+      intros v Hv.
+      rewrite Forall_forall in Hall.
+      apply elem_of_list_lookup in Hv as [k Hv].
+      destruct (decide (k = ka)) as [-> | Hkeq]; cycle 1.
+      + eapply Hall; eauto.
+        {  by apply elem_of_list_lookup_2 in Hv. }
+        eexists k; split; first done.
+        assert (is_Some (l !! k)) as [f Hk].
+        { apply lookup_lt_is_Some_2.
+          eapply lookup_lt_Some in Hv; eauto.
+          rewrite Hlength_mem.
+          done.
+        }
+        assert (f ≠ a).
+        { intros ->.
+          apply Hkeq.
+          eapply NoDup_lookup; eauto.
+          setoid_rewrite Hl.
+          apply finz_seq_between_NoDup.
+        }
+        exists f; split; auto.
+        apply elem_of_list_lookup_2 in Hk.
+        setoid_rewrite Hl in Hk.
+        replace e with (a ^+1)%a in Hk; last solve_addr.
+        apply elem_of_finz_seq_between in Hk.
+        solve_addr.
+      + destruct Hz as (z & Hz); cbn in *.
+        assert ( w = WInt z) ; simplify_eq.
+        { destruct w ; destruct_perm p; done. }
+        rewrite list_lookup_middle in Hv; simplify_eq; first (eexists ; done).
+        rewrite Hlw1; subst la1.
+        rewrite length_take_le; last (eapply Nat.lt_le_incl, lookup_lt_Some; eauto).
+        done.
+    - replace ((a ^+ 1)%a <? e)%Z with true by solve_addr.
+      iInstr "Hcode".
+      { transitivity (Some pc_a); auto; solve_addr. }
+      subst hcont; unfocus_block "Hcode" "Hcont" as "Hcode".
+      iApply ("IH" with "[] [] [$] [$] [$] [$] [$] [$] [$]"); eauto.
+      { iPureIntro; solve_addr. }
+      { iPureIntro.
+        apply Forall_forall.
+        rewrite Forall_forall in Hall.
+        intros v Hv Hk.
+        destruct Hk as (k & Hwk & ak & Hak & Hak_bounds).
+        destruct (decide (ak = a)) as [-> | Ha_ak].
+        + assert (k = ka); simplify_eq.
+          {
+            eapply NoDup_lookup; eauto.
+            setoid_rewrite Hl.
+            apply finz_seq_between_NoDup.
+          }
+          destruct Hz as (z & Hz); cbn in *.
+          assert ( w = WInt z) ; simplify_eq.
+          { destruct w ; destruct_perm p; done. }
+          rewrite list_lookup_middle in Hwk; simplify_eq; first (eexists ; done).
+          rewrite Hlw1; subst la1.
+          rewrite length_take_le; last (eapply Nat.lt_le_incl, lookup_lt_Some; eauto).
+          done.
+        + apply Hall; eauto.
+          exists k; split; auto.
+          exists ak; split; auto.
+          solve_addr.
+      }
+  Qed.
+
+  Lemma checkints_spec
+    (r r1 r2 : RegName)
+    (pc_p : Perm) (pc_g : Locality) (pc_b pc_e pc_a : Addr)
+    (w1 w2 : Word) (l : list Addr) (ws : list Word)
+    (p : Perm) (g : Locality) (b e a : Addr)
+    (φ : language.val cap_lang → iPropI Σ) :
+
+    let checkints := (checkints_instrs r r1 r2) in
+    let a_last := (pc_a ^+ length checkints)%a in
+    executeAllowed pc_p = true →
+    SubBounds pc_b pc_e pc_a a_last →
+    l ≡ₚ (finz.seq_between b e) ->
+    readAllowed p = true ->
+    r ≠ cnull ->
+    r1 ≠ cnull ->
+    r2 ≠ cnull ->
+
+    ▷ PC ↦ᵣ WCap pc_p pc_g pc_b pc_e pc_a
+    ∗ ▷ r ↦ᵣ (WCap p g b e a)
+    ∗ ▷ r1 ↦ᵣ w1
+    ∗ ▷ r2 ↦ᵣ w2
+    ∗ ▷ codefrag pc_a checkints
+    ∗ ▷ ( [∗ list] a;v ∈ l;ws, a ↦ₐ v )
+    ∗ ▷ ( PC ↦ᵣ WCap pc_p pc_g pc_b pc_e a_last
+         ∗ r ↦ᵣ WCap p g b e (finz.max b e)
+         ∗ r1 ↦ᵣ WInt 0%Z
+         ∗ r2 ↦ᵣ WInt 0%Z
+         ∗ ( [∗ list] a;v ∈ l;ws, a ↦ₐ v )
+         ∗ ⌜ Forall (λ w, ∃ z, w = WInt z) ws ⌝
+         ∗ codefrag pc_a checkints
+         ∗ £ 2
+         -∗ WP Seq (Instr Executable) {{ φ }}
+        )
+    ∗ □ (▷ φ FailedV)
+    ⊢ WP Seq (Instr Executable) {{ φ }}.
+  Proof.
+    intros checkints a_last ; subst checkints a_last.
+    iIntros (Hvpc Hcont Hl Hra Hrcnull Hr1cnull Hr2cnull)
+      "(>HPC & >Hr & >Hr1 & >Hr2 & >Hcode & >Hmem & Hφ & #Hfailed)".
+    iDestruct (big_sepL2_length with "Hcode") as %Hlength.
+    iDestruct (big_sepL2_length with "Hmem") as %Hlength_mem
+    ; setoid_rewrite Hl in Hlength_mem.
+    codefrag_facts "Hcode".
+    rename H into HcontRegion; clear H0.
+    rewrite /checkints_instrs.
+
+    focus_block_0 "Hcode" as "Hcode" "Hcont"; iHide "Hcont" as hcont.
+    iApply (lea_to_base_spec with "[- $HPC $Hr $Hr1 $Hr2 $Hcode]"); eauto.
+    iNext; iIntros "(HPC & Hr & Hr1 & Hr2 & Hcode)".
+    subst hcont; unfocus_block "Hcode" "Hcont" as "Hcode".
+
+    focus_block 1 "Hcode" as a_init Ha_init "Hcode" "Hcont"; iHide "Hcont" as hcont.
+    iInstr "Hcode" with "Hlc".
+    iInstr "Hcode" with "Hlc".
+    iInstr "Hcode".
+    iInstr "Hcode".
+    destruct (decide (b < e)%a) as [Hbe|Hbe]; cycle 1.
+    { pose proof Hbe as Hbe'.
+      apply Z.ltb_nlt in Hbe; rewrite Hbe ; cbn.
+      replace (0 - 1%nat)%Z with (-1)%Z by lia.
+      iInstr "Hcode".
+      { transitivity (Some (a_init ^+ 16)%a); auto; solve_addr. }
+      subst hcont; unfocus_block "Hcode" "Hcont" as "Hcode".
+      focus_block 3 "Hcode" as a_end Ha_end "Hcode" "Hcont"; iHide "Hcont" as hcont; clear Ha_init a_init.
+      iInstr "Hcode".
+      iInstr "Hcode".
+      subst hcont; unfocus_block "Hcode" "Hcont" as "Hcode".
+      replace (a_end ^+ 2)%a with (pc_a ^+ 24%nat)%a by solve_addr.
+      replace (finz.max b e) with b by solve_addr.
+      iApply "Hφ"; iFrame; eauto.
+      rewrite finz_seq_between_length finz_dist_0 in Hlength_mem; last solve_addr.
+      symmetry in Hlength_mem. apply nil_length_inv in Hlength_mem; simplify_eq.
+      done.
+    }
+
+    apply Z.ltb_lt in Hbe; rewrite Hbe; cbn.
+    replace (1 - 1%nat)%Z with 0%Z by lia.
+    iInstr "Hcode".
+    subst hcont; unfocus_block "Hcode" "Hcont" as "Hcode".
+    focus_block 2 "Hcode" as a_loop Ha_loop "Hcode" "Hcont"; iHide "Hcont" as hcont
+    ; clear Ha_init a_init.
+    iApply (checkints_loop_spec with "[- $HPC $Hr $Hr1 $Hr2 $Hcode $Hmem]"); eauto.
+    { solve_addr. }
+    { apply Forall_forall.
+      intros v Hv (k & Hkv & (ka & Hka & Hka_bounds)).
+      solve_addr.
+    }
+    iSplitR "Hfailed"; last (iModIntro ; iNext ; iApply "Hfailed").
+    iNext; iIntros "(HPC & Hr & Hr1 & Hr2 & Hmem & % & Hcode)".
+    subst hcont; unfocus_block "Hcode" "Hcont" as "Hcode".
+
+    focus_block 3 "Hcode" as a_end Ha_end "Hcode" "Hcont"; iHide "Hcont" as hcont; clear Ha_loop a_loop.
+    iInstr "Hcode".
+    iInstr "Hcode".
+    subst hcont; unfocus_block "Hcode" "Hcont" as "Hcode".
+    replace (a_end ^+ 2)%a with (pc_a ^+ 24%nat)%a by solve_addr.
+    iApply "Hφ"; iFrame; eauto.
+  Qed.
+
+End Checkints_spec.
