theories/case_studies/macros/checkra.v
@@ -1,0 +1,176 @@
+From iris.proofmode Require Import proofmode.
+From cap_machine Require Import rules proofmode.
+From cap_machine Require Import is_word_type lea_to_base.
+
+Section Checkra.
+  Context
+      {MP: MachineParameters}
+  .
+
+
+  Definition checkra_instrs (r r1 r2 : RegName) : list Word :=
+    encodeInstrsW [
+        GetWType r1 r;
+        Sub r2 r1 (encodeWordType wt_cap);
+        Jnz 4 r2;
+        GetP r1 r;
+        Sub r2 r1 (encodePerm (O LG LM));
+        Jnz 2 r2;
+        Fail;
+        Sub r2 r1 (encodePerm (O DL LM));
+        Jnz 2 r2;
+        Fail;
+        Sub r2 r1 (encodePerm (O LG DRO));
+        Jnz 2 r2;
+        Fail;
+        Sub r2 r1 (encodePerm (O DL DRO));
+        Jnz 2 r2;
+        Fail;
+        Sub r2 r1 (encodePerm WO);
+        Jnz 2 r2;
+        Fail;
+        Sub r2 r1 (encodePerm WO_DL);
+        Jnz 2 r2;
+        Fail;
+        Sub r2 r1 (encodePerm WO_DRO);
+        Jnz 2 r2;
+        Fail;
+        Sub r2 r1 (encodePerm WO_DL_DRO);
+        Jnz 2 r2;
+        Fail;
+        Sub r2 r1 (encodePerm WLO);
+        Jnz 2 r2;
+        Fail;
+        Sub r2 r1 (encodePerm WLO_DL);
+        Jnz 2 r2;
+        Fail;
+        Sub r2 r1 (encodePerm WLO_DRO);
+        Jnz 2 r2;
+        Fail;
+        Sub r2 r1 (encodePerm WLO_DL_DRO);
+        Jnz 2 r2;
+        Fail;
+        Mov r1 0%Z;
+        Mov r2 0%Z ].
+  (* TODO: it's actually quite annoying to check...
+     In CHERIoT, I would do something like:
+     ```
+     GetP r1 r;
+     LAnd r1 (R, Ow, DL, DRO);
+     ```
+
+     Maybe I should have another instruction in the machine
+     for checking this easily?
+   *)
+
+
+End Checkra.
+
+Section Checkra_spec.
+  Context
+    {Σ : gFunctors}
+      {ceriseg: ceriseG Σ}
+      {MP: MachineParameters}
+  .
+
+  Local Ltac fail_check_ra :=
+    match goal with
+    | _ : _ |- context [ WInt (encodePerm ?p - encodePerm ?p') ] =>
+        replace (encodePerm p' - encodePerm p')%Z with 0%Z by lia
+    end
+    ; iInstr "Hcode"
+    ; iInstr "Hcode"
+    ; by wp_end.
+  Local Ltac pass_check_ra :=
+    match goal with
+    | _ : _ |- context [ WInt (encodePerm ?p - encodePerm ?p') ] =>
+        let Heq := fresh "Heq" in
+        let Hneq := fresh "Hneq" in
+        assert ( (WInt (encodePerm p - encodePerm p') ≠ WInt 0 )) as Hneq
+        ; [
+            intro; simplify_eq
+            ; assert (encodePerm p = encodePerm p' ) as Heq by lia
+            ; apply encodePerm_inj in Heq
+            ; done
+          |]
+        ; iInstr "Hcode"
+        ; iInstr "Hcode"
+        ; clear Hneq
+    end.
+  Local Ltac check_ra :=
+    match goal with
+    | _ : _ |- context [ WInt (encodePerm ?p - encodePerm ?p') ] =>
+        let Hp := fresh "Hp" in
+        destruct (decide (p = p')) as [-> | Hp]; [fail_check_ra|pass_check_ra]
+    end.
+
+  Lemma checkra_spec
+    (rsrc r1 r2 : RegName)
+    (pc_p : Perm) (pc_g : Locality) (pc_b pc_e pc_a : Addr)
+    (wsrc w1 w2 : Word)
+    (φ : language.val cap_lang → iPropI Σ) :
+
+    let checkra_ := (checkra_instrs rsrc r1 r2) in
+    let a_last := (pc_a ^+ length checkra_)%a in
+    executeAllowed pc_p = true →
+    SubBounds pc_b pc_e pc_a a_last →
+    rsrc ≠ cnull ->
+    r1 ≠ cnull ->
+    r2 ≠ cnull ->
+
+    ▷ PC ↦ᵣ WCap pc_p pc_g pc_b pc_e pc_a
+    ∗ ▷ rsrc ↦ᵣ wsrc
+    ∗ ▷ r1 ↦ᵣ w1
+    ∗ ▷ r2 ↦ᵣ w2
+    ∗ ▷ codefrag pc_a checkra_
+    ∗ ▷ ( (∃ p g b e a,
+          ⌜ readAllowed p = true ∧ wsrc = WCap p g b e a⌝
+          ∗ PC ↦ᵣ WCap pc_p pc_g pc_b pc_e a_last
+          ∗ rsrc ↦ᵣ WCap p g b e a
+          ∗ r1 ↦ᵣ WInt 0%Z
+          ∗ r2 ↦ᵣ WInt 0%Z
+          ∗ codefrag pc_a checkra_ )
+            -∗ WP Seq (Instr Executable) {{ φ }}
+        )
+    ∗ □ (▷ φ FailedV)
+    ⊢ WP Seq (Instr Executable) {{ φ }}.
+  Proof.
+    intros checkra a_last ; subst checkra a_last.
+    iIntros (Hra Hbounds Hsrc_cnull Hr1_cnull Hr2_cnull) "(>HPC & >Hsrc & >Hr1 & >Hr2 & >Hcode & Hpost & #Hfailed)".
+    codefrag_facts "Hcode".
+    rename H into HcontRegion; clear H0.
+
+    iInstr "Hcode".
+    { rewrite /rules_Get.denote.
+      destruct_word wsrc;done.
+    }
+    iInstr "Hcode".
+
+    destruct (is_cap wsrc) eqn:His_cap_wsrc; cycle 1.
+    { assert (WInt (encodeWordType wsrc - encodeWordType wt_cap)%Z ≠ WInt 0).
+      { intro; simplify_eq.
+        destruct_word wsrc; cbn in *; try done.
+        all: match goal with
+             | _ : ((encodeWordType ?w - encodeWordType wt_cap)%Z = 0%Z) |- _ =>
+                 pose proof (encodeWordType_correct w wt_cap) as Hwtype ; cbn in Hwtype; lia
+             end.
+      }
+      iInstr "Hcode".
+      iInstr "Hcode".
+      by wp_end.
+    }
+    destruct_word wsrc; cbn in His_cap_wsrc; try done.
+    pose proof (encodeWordType_correct (WCap c g b e a) wt_cap) as Hwtype ; cbn in Hwtype.
+    rewrite Hwtype.
+    replace (encodeWordType wt_cap - encodeWordType wt_cap)%Z with 0%Z by lia.
+    iInstr "Hcode".
+    iInstr "Hcode".
+    iInstr "Hcode".
+    do 12 check_ra.
+    iInstr "Hcode".
+    iApply "Hpost"; iFrame.
+    iPureIntro; split; last done.
+    destruct_perm c; auto.
+  Qed.
+
+End Checkra_spec.
