theories/case_studies/macros/is_word_type.v
@@ -1,0 +1,141 @@
+From iris.proofmode Require Import proofmode.
+From cap_machine Require Import rules proofmode.
+
+Section Is_WordType.
+  Context
+      {MP: MachineParameters}
+  .
+
+  Definition is_word_type_instrs (r r1 : RegName) (wtype : Word) : list Word :=
+    encodeInstrsW [
+        GetWType r1 r;
+        Sub r1 r1 (encodeWordType wtype);
+        (* if getwtype(r) == wtype
+           then r1 = 0
+           then r1 != 0
+         *)
+        Jnz 2 r1; (* r2 is zero, then continue, else jump to fail *)
+        (* getwtype(r) == wtype *)
+        Jmp 2;
+        (* getwtype(r) != wtype *)
+        Fail
+      ].
+
+  Definition is_int_instrs (r r1 : RegName) : list Word :=
+   is_word_type_instrs r r1 wt_int.
+  Definition is_memory_cap_instrs (r r1 : RegName) : list Word :=
+   is_word_type_instrs r r1 wt_cap.
+End Is_WordType.
+
+Section Is_WordType_spec.
+  Context
+    {Σ : gFunctors}
+      {ceriseg: ceriseG Σ}
+      {MP: MachineParameters}
+  .
+
+  Lemma is_int_spec
+    (r r1 : RegName)
+    (pc_p : Perm) (pc_g : Locality) (pc_b pc_e pc_a : Addr)
+    (w w1 wtype : Word)
+    (φ : language.val cap_lang → iPropI Σ) :
+
+    let is_int := (is_int_instrs r r1) in
+    let a_last := (pc_a ^+ length is_int)%a in
+    executeAllowed pc_p = true →
+    SubBounds pc_b pc_e pc_a a_last →
+    r ≠ cnull ->
+    r1 ≠ cnull ->
+
+    ▷ PC ↦ᵣ WCap pc_p pc_g pc_b pc_e pc_a
+    ∗ ▷ r ↦ᵣ w
+    ∗ ▷ r1 ↦ᵣ w1
+    ∗ ▷ codefrag pc_a is_int
+    ∗ ▷ ( ( PC ↦ᵣ WCap pc_p pc_g pc_b pc_e a_last
+            ∗ r ↦ᵣ w ∗ ⌜ ∃ z, w = WInt z ⌝
+            ∗ r1 ↦ᵣ WInt 0%Z
+            ∗ codefrag pc_a is_int)
+              -∗ WP Seq (Instr Executable) {{ φ }}
+        )
+    ∗ ▷ φ FailedV
+    ⊢ WP Seq (Instr Executable) {{ φ }}.
+  Proof.
+    intros is_int a_last ; subst is_int a_last.
+    iIntros (Hvpc Hcont Hrcnull Hr1cnull)
+      "(>HPC & >Hr & >Hr1 & >Hprog & Hφ & Hfailed)".
+    iDestruct (big_sepL2_length with "Hprog") as %Hlength.
+    codefrag_facts "Hprog".
+    rename H into HcontRegion; clear H0.
+    destruct (is_z w) eqn:Hw_z.
+    - destruct w; cbn in *; try done.
+      iInstr "Hprog".
+      iInstr "Hprog".
+      replace (encodeWordType (WInt z) - encodeWordType wt_int)%Z with 0%Z.
+      2: { rewrite (encodeWordType_correct_int z 0) /wt_int; lia. }
+      iGo "Hprog".
+      iApply "Hφ"; iFrame.
+      iPureIntro; eexists; done.
+    - iGo "Hprog".
+      { apply getwtype_denote. }
+      assert (WInt (encodeWordType w - encodeWordType wt_int) ≠ WInt 0).
+      { pose proof (encodeWordType_correct w wt_int) as Hencode ; cbn in Hencode.
+        intro H; injection H; intro Hcontra.
+        destruct w as [| [] | |]; cbn in *; try done; try lia.
+      }
+      iGo "Hprog".
+      wp_end; iApply "Hfailed".
+  Qed.
+
+  Lemma is_memory_cap_spec
+    (r r1 : RegName)
+    (pc_p : Perm) (pc_g : Locality) (pc_b pc_e pc_a : Addr)
+    (w w1 wtype : Word)
+    (φ : language.val cap_lang → iPropI Σ) :
+
+    let is_memory_cap := (is_memory_cap_instrs r r1) in
+    let a_last := (pc_a ^+ length is_memory_cap)%a in
+    executeAllowed pc_p = true →
+    SubBounds pc_b pc_e pc_a a_last →
+    r ≠ cnull ->
+    r1 ≠ cnull ->
+
+    ▷ PC ↦ᵣ WCap pc_p pc_g pc_b pc_e pc_a
+    ∗ ▷ r ↦ᵣ w
+    ∗ ▷ r1 ↦ᵣ w1
+    ∗ ▷ codefrag pc_a is_memory_cap
+    ∗ ▷ ( (∃ p g b e a,
+            PC ↦ᵣ WCap pc_p pc_g pc_b pc_e a_last
+            ∗ r ↦ᵣ WCap p g b e a
+            ∗ r1 ↦ᵣ WInt 0%Z
+            ∗ codefrag pc_a is_memory_cap)
+              -∗ WP Seq (Instr Executable) {{ φ }}
+        )
+    ∗ ▷ φ FailedV
+    ⊢ WP Seq (Instr Executable) {{ φ }}.
+  Proof.
+    intros is_int a_last ; subst is_int a_last.
+    iIntros (Hvpc Hcont Hrcnull Hr1cnull)
+      "(>HPC & >Hr & >Hr1 & >Hprog & Hφ & Hfailed)".
+    iDestruct (big_sepL2_length with "Hprog") as %Hlength.
+    codefrag_facts "Hprog".
+    rename H into HcontRegion; clear H0.
+    destruct (is_cap w) eqn:Hw_cap.
+    - destruct_word w; cbn in *; try done.
+      iInstr "Hprog".
+      iInstr "Hprog".
+      replace (encodeWordType (WCap c g b e a) - encodeWordType wt_cap)%Z with 0%Z.
+      2: { rewrite (encodeWordType_correct_cap c g b e a (O LG LM) Global 0%a 0%a 0%a) /wt_cap; lia. }
+      iGo "Hprog".
+      iApply "Hφ"; iFrame.
+    - iGo "Hprog".
+      { apply getwtype_denote. }
+      assert (WInt (encodeWordType w - encodeWordType wt_cap) ≠ WInt 0).
+      { pose proof (encodeWordType_correct w wt_cap) as Hencode ; cbn in Hencode.
+        intro H; injection H; intro Hcontra.
+        destruct w as [| [] | |]; cbn in *; try done; try lia.
+      }
+      iGo "Hprog".
+      wp_end; iApply "Hfailed".
+  Qed.
+
+End Is_WordType_spec.
