theories/utils/stdpp_extra.v
@@ -1031,6 +1031,53 @@ Proof.
 Qed.
 
 
+Class DisjointList A := disjoint_list : list A → Prop.
+#[export] Hint Mode DisjointList ! : typeclass_instances.
+Instance: Params (@disjoint_list) 2 := {}.
+Notation "## Xs" := (disjoint_list Xs) (at level 20, format "##  Xs") : stdpp_scope.
+Notation "##@{ A } Xs" :=
+  (@disjoint_list A _ Xs) (at level 20, only parsing) : stdpp_scope.
+
+Section disjoint_list.
+  Variable A: Type.
+  Context `{Disjoint A, Union A, Empty A}.
+  Implicit Types X : A.
+
+  Inductive disjoint_list_default : DisjointList A :=
+    | disjoint_nil_2 : ##@{A} []
+    | disjoint_cons_2 (X : A) (Xs : list A) : X ## ⋃ Xs → ## Xs → ## (X :: Xs).
+  Global Existing Instance disjoint_list_default.
+
+  Lemma disjoint_list_nil  : ##@{A} [] ↔ True.
+  Proof. split; constructor. Qed.
+  Lemma disjoint_list_cons X Xs : ## (X :: Xs) ↔ X ## ⋃ Xs ∧ ## Xs.
+  Proof.
+    split; [inversion_clear 1; auto |].
+    intros [??]. constructor; auto.
+  Qed.
+End disjoint_list.
+
+Lemma disjoint_mono_l A C `{ElemOf A C} (X Y Z: C) : X ⊆ Y → Y ## Z → X ## Z.
+Proof. intros * HXY. rewrite !elem_of_disjoint. eauto. Qed.
+
+Lemma disjoint_mono_r A C `{ElemOf A C} (X Y Z: C) : X ⊆ Y → Z ## Y → Z ## X.
+Proof. intros * HXY. rewrite !elem_of_disjoint. eauto. Qed.
+
+Global Instance Empty_list {A}: Empty (list A). exact []. Defined.
+Global Instance Union_list {A}: Union (list A). exact app. Defined.
+Global Instance Singleton_list {A}: Singleton A (list A). exact (λ a, [a]). Defined.
+Global Instance Semiset_list {A}: SemiSet A (list A) .
+Proof. split; set_solver. Qed.
+
+Lemma filter_complement_list {A : Type} (l : list A) (P : A -> Prop) {Hdec: ∀ x, Decision (P x)} :
+  l ≡ₚ filter P l ∪ filter (λ x : A, ¬ P x) l.
+Proof.
+  induction l; cbn; first done.
+  rewrite /union /Union_list.
+  destruct ( decide (P a) ); destruct ( decide (¬ P a) ); try done.
+  + rewrite -app_comm_cons {1}IHl; done.
+  + rewrite -Permutation_middle {1}IHl; done.
+Qed.
 
 Definition prod_op {A B : Type} :=
   λ (o1 : option A) (o2 : option B),
